Martin Escardo, Vincent Rahli, Bruno da Rocha Paiva, Ayberk Tosun 20 May 2023

We prove the correctness of the internal translation.

\begin{code}

{-# OPTIONS --safe --without-K --exact-split #-}

module EffectfulForcing.Internal.Correctness where

open import MLTT.Spartan hiding (rec ; _^_) renaming (⋆ to 〈〉)
open import EffectfulForcing.MFPSAndVariations.Combinators
open import EffectfulForcing.MFPSAndVariations.Continuity
open import EffectfulForcing.MFPSAndVariations.Dialogue
open import EffectfulForcing.MFPSAndVariations.SystemT using (type ; ι ; _⇒_ ; 〖_〗)
open import EffectfulForcing.MFPSAndVariations.LambdaCalculusVersionOfMFPS
                              using (B〖_〗 ; Kleisli-extension ; zero' ; succ' ; rec')
open import EffectfulForcing.MFPSAndVariations.Church
                              hiding (B⋆【_】 ; ⟪⟫⋆ ; _‚‚⋆_ ; B⋆⟦_⟧ ; dialogue-tree⋆)
open import EffectfulForcing.Internal.Internal hiding (B⋆⟦_⟧ ; dialogue-tree⋆)
open import EffectfulForcing.Internal.External
open import EffectfulForcing.Internal.SystemT
open import EffectfulForcing.Internal.Subst
open import UF.Base using (transport₂ ; transport₃ ; ap₂ ; ap₃)

\end{code}

Using a logical relation we show that the the internal, church-encoded dialogue
translation of a System T term coincides with its external, inductive dialogue
translation.

From this result and the main-lemma we can derive an internal result of
strong continuity in System T.

\begin{code}

is-dialogue-for : B ℕ → ({A : type} → T₀ (B-type〖 ι 〗 A)) → Type
is-dialogue-for d t = {A : type} → ⟦ t ⟧₀ ≡[ B-type〖 ι 〗 A ] church-encode d

-- Logical relation for internal dialogue trees which can be pattern matched on
-- and for functions that preserve said pattern matching.
Rnorm : {σ : type} (d : B〖 σ 〗) (t : {A : type} → T₀ (B-type〖 σ 〗 A)) → Type
Rnorm {ι}     d t = is-dialogue-for d t
Rnorm {σ ⇒ τ} d t = (u : B〖 σ 〗) (u' : {A : type} → T₀ (B-type〖 σ 〗 A))
                  → Rnorm u u' → Rnorm (d u) (t · u')

-- internal semantics of contexts as dialogue trees
IB【_】 : Cxt → type → Type
IB【 Γ 】 A = Sub₀ (B-context【 Γ 】 A)

Rnorms : {Γ : Cxt} → B【 Γ 】 → ({A : type} → IB【 Γ 】 A) → Type
Rnorms {Γ} xs ys = {σ : type} (i : ∈Cxt σ Γ) → Rnorm (xs i) (ys (∈Cxt-B-type i))

-- To avoid the operational semantics, we use the following lemma.
Rnorm-respects-≡ : {σ : type} {d : B〖 σ 〗} {t u : {A : type} → T₀ (B-type〖 σ 〗 A)}
                   → ({A : type} → ⟦ t ⟧₀ ≡[ (B-type〖 σ 〗 A) ] ⟦ u ⟧₀)
                   → Rnorm d t
                   → Rnorm d u
Rnorm-respects-≡ {ι} {d} {t} {u} t≡u Rnorm-d-t {A} {η₁} {η₂} η₁≡η₂ {β₁} {β₂} β₁≡β₂ =
 ⟦ u ⟧₀ η₁ β₁          ≡⟨ ≡-symm (t≡u {A} (≡ₗ η₁ η₁≡η₂) (≡ₗ β₁ β₁≡β₂)) ⟩
 ⟦ t ⟧₀ η₁ β₁          ≡＝⟨ Rnorm-d-t η₁≡η₂ β₁≡β₂ ⟩
 church-encode d η₂ β₂ ∎
Rnorm-respects-≡ {σ ⇒ τ} {d} {t} {u} t≡u Rnorm-t v₁ v₂ Rnorm-vs =
 Rnorm-respects-≡ -- (d v₁) (t · v₂) (u · v₂)
                    (t≡u (≡-refl₀ v₂))
                    (Rnorm-t v₁ v₂ Rnorm-vs)

\end{code}

As Rnorm quantifies over all System T types, we can elimate a family of
church-encoded trees into different types, allowing us to reify terms into
the shape of ⌜η⌝ or ⌜β⌝.

This sort of reification is crucial when we need to pattern match on the
constructor of a church-encoded tree.

Require fact that Rnorm is parametric when proving the reflects-≡ lemmas.

\begin{code}

-- TODO this should be moved to the definition of numeral?
⟦numeral⟧ : {Γ : Cxt} (γ : 【 Γ 】) (n : ℕ) → ⟦ numeral n ⟧ γ ≡ n
⟦numeral⟧ γ  zero    = refl
⟦numeral⟧ γ (succ n) = ap succ (⟦numeral⟧ γ n)

⟦numeral⟧₀ : (n : ℕ) → ⟦ numeral n ⟧₀ ＝ n
⟦numeral⟧₀  n = ⟦numeral⟧ ⟨⟩ n

Rnorm-numeral : (n : ℕ) → Rnorm (η n) (⌜η⌝ · numeral n)
Rnorm-numeral n η₁≡η₂ β₁≡β₂ = η₁≡η₂ (⟦numeral⟧₀ n)

Rnorm-η-implies-≡ : {n₁ : ℕ} {n₂ : T₀ ι}
                  → Rnorm (η n₁) (⌜η⌝ · n₂)
                  → ⟦ numeral n₁ ⟧₀ ≡ ⟦ n₂ ⟧₀
Rnorm-η-implies-≡ {n₁} {n₂} Rnorm-ns =
 ⟦ numeral n₁ ⟧₀ ≡⟨ ⟦numeral⟧₀ n₁ ⟩
 n₁              ≡⟨ ≡-symm (Rnorm-ns η₁≡η₁ β₁≡β₁) ⟩
 ⟦ n₂ ⟧₀ ∎
 where
  η₁ : ℕ → ℕ
  η₁ n = n

  η₁≡η₁ : η₁ ≡ η₁
  η₁≡η₁ n₁＝n₂ = n₁＝n₂

  β₁ : (ℕ → ℕ) → ℕ → ℕ
  β₁ ϕ n = 0

  β₁≡β₁ : β₁ ≡ β₁
  β₁≡β₁ ϕ₁≡ϕ₂ n₁≡n₂ = refl

-- TODO give this a better name

η-type : type → type
η-type A = ι ⇒ A

β-type : type → type
β-type A = (ι ⇒ A) ⇒ ι ⇒ A

branch : ({A : type} → T₀ (⌜B⌝ ι A)) → {A : type} → T₀ (ι ⇒ ⌜B⌝ ι A)
branch t {A} =
 -- λ i. λ η. λ β. t η' β' h
 ƛ (ƛ (ƛ (weaken₀ (t {A'}) · η' · β' · h)))
 where
  -- To pull out the branching ϕ we use the following elimination type
  A' : type
  A' = β-type A ⇒ A

  -- λ n. λ k. η(n)
  η' : T (〈〉 ,, ι ,, η-type A ,, β-type A) (η-type A')
  η' = ƛ (ƛ (ν₃ · ν₁))

  -- λ g. λ n. λ h. h (λ j. g j β) n
  β' : T (〈〉 ,, ι ,, η-type A ,, β-type A) (β-type A')
  β' = ƛ (ƛ (ƛ (ν₀ · ƛ (ν₃ · ν₀ · ν₄) · ν₁)))

  -- λ k. λ n.k i
  h : T (〈〉 ,, ι ,, η-type A ,, β-type A) (β-type A)
  h = ƛ (ƛ (ν₁ · ν₄))

-- TODO can this proof be tidied at all?
Rnorm-branch : {ϕ : ℕ → B ℕ} {n : ℕ} {t : {A : type} → T₀ (⌜B⌝ ι A)} (i : ℕ)
               → Rnorm (β ϕ n) t
               → Rnorm (ϕ i) (branch t · numeral i)
               --→ ⟦ branch t · numeral i⟧ i ≡ church-encode (ϕ i)
Rnorm-branch {ϕ} {n} {t} i Rnorm-βt {A} {η₁} {η₂} η₁≡η₂ {β₁} {β₂} β₁≡β₂ =
 ⟦ branch t · numeral i ⟧₀ η₁ β₁                        ＝≡⟨ refl ⟩
 ⟦ weaken₀ t ⟧ (⟨⟩ ‚ ⟦ numeral i ⟧₀ ‚ η₁ ‚ β₁) η₀ β₀ h₀ ≡⟨ I η₀≡η₀ β₀≡β₀ h₀≡h₁ ⟩
 church-encode (β ϕ n) η₀ β₀ h₁                         ＝≡⟨ refl ⟩
 church-encode (ϕ i) η₀ β₀ β₁                           ≡＝⟨ q (ϕ i) ⟩
 church-encode (ϕ i) η₂ β₂                              ∎
 where
  -- To pull out the branching ϕ we use the following elimination type
  A' : type
  A' = β-type A ⇒ A

  I : ⟦ weaken₀ (t {A'}) ⟧ (⟨⟩ ‚ ⟦ numeral i ⟧₀ ‚ η₁ ‚ β₁) ≡ church-encode (β ϕ n)
  I = ≡-trans {⌜B⌝ ι _} (⟦weaken₀⟧ t ((⟨⟩ ‚ ⟦ numeral i ⟧ ⟨⟩ ‚ η₁ ‚ β₁))) Rnorm-βt

  η₀ : 〖 η-type A' 〗
  η₀ = λ n → λ k → η₁ n

  η₀≡η₀ : η₀ ≡ η₀
  η₀≡η₀ n₁≡n₂ k₁≡k₂ = ≡ₗ η₁ η₁≡η₂ n₁≡n₂

  β₀ : 〖 β-type A' 〗
  β₀ = λ g → λ n → λ h → h (λ j → g j β₁) n

  β₀≡β₀ : β₀ ≡ β₀
  β₀≡β₀ g₁≡g₂ n₁≡n₂ h₁≡h₂ = h₁≡h₂ (λ j₁≡j₂ → g₁≡g₂ j₁≡j₂ (≡ₗ β₁ β₁≡β₂)) n₁≡n₂

  h₀ : 〖 β-type A 〗
  h₀ = λ k → λ n → k ⟦ numeral i ⟧₀

  h₁ : 〖 β-type A 〗
  h₁ = λ k → λ n → k i

  h₀≡h₁ : h₀ ≡ h₁
  h₀≡h₁ k₁≡k₂ n₁≡n₂ = k₁≡k₂ (⟦numeral⟧₀ i)

  q : (d : B ℕ) → church-encode d η₀ β₀ β₁ ≡ church-encode d η₂ β₂
  q (η x)   = η₁≡η₂ refl
  q (β ψ y) = β₁≡β₂ ψ≡ψ refl
   where
    ψ≡ψ : (λ i → church-encode (ψ i) η₀ β₀ β₁) ≡ (λ i → church-encode (ψ i) η₂ β₂)
    ψ≡ψ {j} {.j} refl = q (ψ j)

Rnorm-β-implies-Rnorm-ϕ : {ϕ₁ : ℕ → B ℕ} {n₁ : ℕ}
                          {ϕ₂ : {A : type} → T₀ (ι ⇒  ⌜B⌝ ι A)} {n₂ : T₀ ι}
                          (i : ℕ)
                        → Rnorm (β ϕ₁ n₁) (⌜β⌝ · ϕ₂ · n₂)
                        → Rnorm (ϕ₁ i) (ϕ₂ · numeral i)
Rnorm-β-implies-Rnorm-ϕ = {!!}

Rnorm-β-implies-n-≡ : {ϕ₁ : ℕ → B ℕ} {n₁ : ℕ}
                      {ϕ₂ : {A : type} → T₀ (ι ⇒ ⌜B⌝ ι A)} {n₂ : T₀ ι}
                    → Rnorm (β ϕ₁ n₁) (⌜β⌝ · ϕ₂ · n₂)
                    → ⟦ numeral n₁ ⟧₀ ≡ ⟦ n₂ ⟧₀
Rnorm-β-implies-n-≡ = {!!}

Rnorm-reify-β : (ϕ : ℕ → B ℕ) (n : ℕ) (t : {A : type} → T₀ (⌜B⌝ ι A))
                → Rnorm (β ϕ n) t
                → Σ ϕ' ꞉ ({A : type} → T₀ (ι ⇒ ⌜B⌝ ι A))                -- branch
                , Σ n' ꞉ T₀ ι                                           -- numeral
                , ({A : type} → ⟦ t ⟧₀ ≡[ ⌜B⌝ ι A ] ⟦ ⌜β⌝ · ϕ' · n' ⟧₀) -- follows (almost?) directly from assumption that Rnorm (β ϕ n) t, does it not?
                × Rnorm (β ϕ n) (⌜β⌝ · ϕ' · n')                         -- Rnorm-branch
                × (⟦ n' ⟧₀ ≡ n)                                         -- Rnorm-β-implies-n-≡
                × ((x : ℕ) → Rnorm (ϕ x) (ϕ' · numeral x))              -- Rnorm-β-implies-Rnorm-ϕ
Rnorm-reify-β = {!!}
-- where
--  -- We get the branching at t with the following
--  ϕ' : {A : type} → T₀ (ι ⇒ ⌜B⌝ ι A)
--  ϕ' {A} = B-branch t
--
--  -- We get the oracle query at t with the following
--  n' : T₀ ι
--  n' = numeral n
--
--  eq' : ⟦ t ⟧₀ ≣⋆ ⟦ ⌜β⌝ · ϕ' · n' ⟧₀
--  eq' A η' β' eη eβ =
--   ⟦ t ⟧₀ η' β'
--    ≡⟨ eq A η' β' eη eβ ⟩
--   β' (λ y → church-encode (ϕ y) η' β') n
--    ≡＝⟨ eβ _ _ _ _ ((⟦numeral⟧ n) ⁻¹) (λ y → ≡-symm (⟦B-branch⟧ ϕ y n t eq A η' β' eη eβ)) ⟩
--   ⟦ ⌜β⌝ · ϕ' · n' ⟧₀ η' β'
--    ∎
--
--  rβ : Rnorm (β ϕ n) (⌜β⌝ · ϕ' · n')
--  rβ = ≣⋆-trans (≣⋆-symm eq') eq
--
--  rϕ : (x : ℕ) → ⟦ B-branch t ⟧₀ ⟦ numeral x ⟧₀ ≣⋆ church-encode (ϕ x)
--  rϕ x = transport (λ k → ⟦ B-branch t ⟧₀ k ≣⋆ church-encode (ϕ x))
--                   (⟦numeral⟧ x ⁻¹) (⟦B-branch⟧ ϕ x n t eq)
--
-- TODO: can we generalize this?
church-encode-kleisli-extension : {A : type} (d : B ℕ)
                                → (f₁ : ℕ → B ℕ) (f₂ : {A : type} → T₀ (ι ⇒ ⌜B⌝ ι A))
                                → ((i : ℕ) → Rnorm (f₁ i) (f₂ · numeral i))
                                → church-encode (kleisli-extension f₁ d)
                                  ≡[ ⌜B⌝ ι A ] kleisli-extension⋆ ⟦ f₂ ⟧₀ (church-encode d)
church-encode-kleisli-extension {A} (η n) f₁ f₂ f₁≡f₂ =
 church-encode (f₁ n)                             ≡⟨ ≡-symm {⌜B⌝ ι A} (f₁≡f₂ n) ⟩
 ⟦ f₂ ⟧₀ ⟦ numeral n ⟧₀                           ≡＝⟨ ≡-refl₀ f₂ (⟦numeral⟧₀ n) ⟩
 kleisli-extension⋆ ⟦ f₂ ⟧₀ (church-encode (η n)) ∎
church-encode-kleisli-extension {A} (β ϕ n) f₁ f₂ f₁≡f₂ {η₁} {η₂} η₁≡η₂ {β₁} {β₂} β₁≡β₂ =
 β₁≡β₂ ϕ₁≡ϕ₂ refl
 where
  ϕ₁ : ℕ → 〖 A 〗
  ϕ₁ i = church-encode (kleisli-extension f₁ (ϕ i)) η₁ β₁

  ϕ₂ : ℕ → 〖 A 〗
  ϕ₂ i = kleisli-extension⋆ ⟦ f₂ ⟧₀ (church-encode (ϕ i)) η₂ β₂

  ϕ₁≡ϕ₂ : ϕ₁ ≡ ϕ₂
  ϕ₁≡ϕ₂ {i} {.i} refl = church-encode-kleisli-extension (ϕ i) f₁ f₂ f₁≡f₂ η₁≡η₂ β₁≡β₂

-- TODO maybe move this?
⟦⌜Kleisli-extension⌝⟧ : {X A σ : type} {Γ Δ : Cxt} (xs : 【 Γ 】) (ys : 【 Δ 】)
                      → ⟦ ⌜Kleisli-extension⌝ {X} {A} {σ} ⟧ xs
                      ≡ ⟦ ⌜Kleisli-extension⌝ {X} {A} {σ} ⟧ ys
⟦⌜Kleisli-extension⌝⟧ {X} {A} {ι} {Γ} {Δ} xs ys d₁≡d₂ f₁≡f₂ η₁≡η₂ β₁≡β₂ =
 f₁≡f₂ (λ x₁≡x₂ → d₁≡d₂ x₁≡x₂ η₁≡η₂ β₁≡β₂) β₁≡β₂
⟦⌜Kleisli-extension⌝⟧ {X} {A} {σ ⇒ τ} {Γ} {Δ} xs ys g₁≡g₂ f₁≡f₂ x₁≡x₂ =
 ⟦⌜Kleisli-extension⌝⟧ _ _ (λ y₁≡y₂ → g₁≡g₂ y₁≡y₂ x₁≡x₂) f₁≡f₂

-- Recursion in System T is interpreted by the internal dialogue tree translation
-- using ⌜Kleisli-extension⌝, so to prove the fundamental theorem of Rnorm we
-- need to know that ⌜Kleisli-extension⌝ preserves Rnorm.
Rnorm-kleisli-lemma : {σ : type}

                      (f₁ : ℕ → B〖 σ 〗)
                      (f₂ : {A : type} → T₀ (ι ⇒ B-type〖 σ 〗 A))
                    → ((x : ℕ) → Rnorm (f₁ x) (f₂ · numeral x))

                    → (n₁ : B ℕ)
                      (n₂ : {A : type} → T₀ (⌜B⌝ ι A))
                    → Rnorm {ι} n₁ n₂

                    → Rnorm (Kleisli-extension f₁ n₁) (⌜Kleisli-extension⌝ · f₂ · n₂)
Rnorm-kleisli-lemma {ι} f₁ f₂ Rnorm-fs n₁ n₂ Rnorm-ns {A} =
 ⟦ ⌜kleisli-extension⌝ · f₂ · n₂ ⟧₀
  ≡⟨ ≡-refl₀ {⌜B⌝ ι A ⇒ ⌜B⌝ ι A} (⌜kleisli-extension⌝ · f₂) Rnorm-ns ⟩
 kleisli-extension⋆ ⟦ f₂ ⟧₀ (church-encode n₁)
  ≡＝⟨ ≡-symm {⌜B⌝ ι A} (church-encode-kleisli-extension n₁ f₁ f₂ Rnorm-fs) ⟩
 church-encode (kleisli-extension f₁ n₁)
  ∎
Rnorm-kleisli-lemma {σ ⇒ τ} f₁ f₂ Rnorm-fs n₁ n₂ Rnorm-ns u₁ u₂ Rnorm-us =
 Rnorm-respects-≡ I IH
 where
  -- We perform some computation steps using the semantics.
  I : {A : type}
    → ⟦ ⌜Kleisli-extension⌝ · ƛ (weaken₀ f₂ · ν₀ · weaken₀ u₂) · n₂ ⟧₀
      ≡[ B-type〖 τ 〗 A ] ⟦ ƛ (ƛ (ƛ (⌜Kleisli-extension⌝ · ƛ (ν₃ · ν₀ · ν₁) · ν₁))) · f₂ · n₂ · u₂ ⟧₀
  I = ⟦⌜Kleisli-extension⌝⟧ ⟨⟩ (⟨⟩ ‚ ⟦ f₂ ⟧₀ ‚ ⟦ n₂ ⟧₀ ‚ ⟦ u₂ ⟧₀)
       (λ x₁≡x₂ → ⟦weaken₀⟧ f₂ _ x₁≡x₂ (⟦weaken₀⟧ u₂ _))
       (≡-refl₀ n₂)

  II : (x : ℕ) {A : type}
     → ⟦ ƛ (weaken₀ f₂ · ν₀ · weaken₀ u₂) · numeral x ⟧₀
       ≡[ B-type〖 τ 〗 A ] ⟦ f₂ · numeral x · u₂ ⟧₀
  II x = ⟦weaken₀⟧ f₂ (⟨⟩ ‚ ⟦ numeral x ⟧ ⟨⟩) refl (⟦weaken₀⟧ u₂ (⟨⟩ ‚ ⟦ numeral x ⟧₀))

  -- In the recursive case, Kleisli-extension calls Kleisli-extension at
  -- the codomain type with the following new fs'.
  f₁' : ℕ → B〖 τ 〗
  f₁' x = f₁ x u₁

  f₂' : {A : type} → T₀ (ι ⇒ B-type〖 τ 〗 A)
  f₂' = ƛ (weaken₀ f₂ · ν₀ · weaken₀ u₂)

  -- Crucially, these fs' are still related by Rnorm, so we can use them to get
  -- the inductive hypothesis IH.
  Rnorm-fs' : (x : ℕ) → Rnorm (f₁' x) (f₂' · numeral x)
  Rnorm-fs' x = Rnorm-respects-≡ (≡-symm (II x)) (Rnorm-fs x u₁ u₂ Rnorm-us)

  IH : Rnorm (Kleisli-extension f₁' n₁) (⌜Kleisli-extension⌝ · f₂' · n₂)
  IH = Rnorm-kleisli-lemma f₁' f₂' Rnorm-fs' n₁ n₂ Rnorm-ns


-- TODO is it possible to prove this in general?
-- We could when using ≣⋆ but it seems it would only be true when
-- g : ℕ → ℕ now that we are using ≡
church-encode-is-natural : {g₁ g₂ :  ℕ → ℕ} (d : B ℕ)
                         → g₁ ≡ g₂
                         → {A : type}
                         → B⋆-functor g₁ (church-encode d)
                           ≡[ ⌜B⌝ ι A ] church-encode (B-functor g₂ d)
church-encode-is-natural (η n) g₁≡g₂ {A} η₁≡η₂ β₁≡β₂ = η₁≡η₂ (g₁≡g₂ refl)
church-encode-is-natural {g₁} {g₂} (β ϕ n) g₁≡g₂ {A} {η₁} {η₂} η₁≡η₂ {β₁} {β₂} β₁≡β₂ =
 β₁≡β₂ ϕ₁≡ϕ₂ refl
 where
  ϕ₁ : ℕ → 〖 A 〗
  ϕ₁ i = B⋆-functor g₁ (church-encode (ϕ i)) η₁ β₁

  ϕ₂ : ℕ → 〖 A 〗
  ϕ₂ i = church-encode (B-functor g₂ (ϕ i)) η₂ β₂

  ϕ₁≡ϕ₂ : ϕ₁ ≡ ϕ₂
  ϕ₁≡ϕ₂ {i} {.i} refl = church-encode-is-natural (ϕ i) g₁≡g₂ η₁≡η₂ β₁≡β₂

-- TODO consider moving the compute lemmas to somewhere else?
compute-Rec-Zero : {A σ : type} {Γ : Cxt}
                   (a : T (Γ ,, ι) (ι ⇒ B-type〖 σ ⇒ σ 〗 A))
                   (b : T Γ (B-type〖 σ 〗 A))
                   (s : Sub₀ Γ)
                 → ⟦ (close (ƛ (Rec a (weaken, ι b) ν₀)) s) · Zero ⟧₀
                   ≡ ⟦ close b s ⟧₀
compute-Rec-Zero {A} {σ} {Γ} a b s =
 ⟦ (close (ƛ (Rec a (weaken, ι b) ν₀)) s) · Zero ⟧₀
  ＝≡⟨ refl ⟩
 ⟦ close (weaken, ι b) (Subƛ s) ⟧ (⟨⟩ ‚ zero)
  ＝≡⟨ ap (λ k → ⟦ k ⟧ (⟨⟩ ‚ zero)) (close-weaken b (⊆, Γ ι) (Subƛ s)) ⟩
 ⟦ close b (⊆Sub (∈CxtS ι) (Subƛ s)) ⟧ (⟨⟩ ‚ zero)
  ≡⟨ ⟦close⟧ b (⊆Sub (∈CxtS ι) (Subƛ s)) _ _ (【≡】-is-refl‚ _ _ (λ ()) refl) (【≡】-【Sub】-⊆Sub' s) ⟩
 ⟦ b ⟧ (【Sub】 (⊆Sub (∈CxtS ι) (Subƛ s)) (⟨⟩ ‚ zero))
  ≡⟨ ≡-refl b (【≡】-【Sub】-⊆Sub s) ⟩
 ⟦ b ⟧ (【Sub₀】 s)
  ≡＝⟨ ≡-symm (⟦close⟧ b s _ _ (λ ()) (【≡】-is-refl-【Sub₀】 s)) ⟩
 ⟦ close b s ⟧₀
  ∎

compute-Rec-Succ : {A σ : type} {Γ : Cxt}
                       (a : T Γ (B-type〖 ι ⇒ σ ⇒ σ 〗 A))
                       (b : T Γ (B-type〖 σ 〗 A))
                       (n : T₀ ι)
                       (s : Sub₀ Γ)
                     → ⟦ close (ƛ (Rec (ƛ (weaken, ι (weaken, ι a) · (⌜η⌝ · ν₀))) (weaken, ι b) ν₀)) s · Succ n ⟧₀
                     ≡ ⟦ close a s · (⌜η⌝ · n) · Rec (ƛ (weaken, ι (close a s) · (⌜η⌝ · ν₀))) (close b s) n ⟧₀
compute-Rec-Succ {A} {σ} {Γ} a b n s =
 ⟦ close (ƛ (Rec (ƛ (weaken, ι (weaken, ι a) · (⌜η⌝ · ν₀))) (weaken, ι b) ν₀)) s · Succ n ⟧₀
  ＝≡⟨ refl ⟩
 ⟦ close (weaken, ι (weaken, ι a)) (Subƛ (Subƛ s)) ⟧ (⟨⟩ ‚ succ ⟦ n ⟧₀ ‚ ⟦ n ⟧₀)
  (η⋆ ⟦ n ⟧₀)
  (rec (λ x → ⟦ close (weaken, ι (weaken, ι a) · (⌜η⌝ · ν₀)) (Subƛ (Subƛ s)) ⟧ (⟨⟩ ‚ succ ⟦ n ⟧₀ ‚ x))
       (⟦ close (weaken, ι b) (Subƛ s) ⟧ (⟨⟩ ‚ succ ⟦ n ⟧₀))
       ⟦ n ⟧₀)
  --≡＝⟨ e1 _ _ (λ a₁ b₁ a≡₁ a₂ b₂ a≡₂ → a≡₁ _ _ refl) _ _ e2 ⟩
  ≡＝⟨ {!!} ⟩
 ⟦ close a s ⟧₀
  (η⋆ ⟦ n ⟧₀)
  (rec ⟦ ƛ (weaken, ι (close a s) · (⌜η⌝ · ν₀)) ⟧₀ ⟦ close b s ⟧₀ ⟦ n ⟧₀)
  ＝⟨ refl ⟩
 ⟦ close a s · (⌜η⌝ · n) · Rec (ƛ (weaken, ι (close a s) · (⌜η⌝ · ν₀))) (close b s) n ⟧₀
  ∎
 where
  e0 : {τ : type} (i : ∈Cxt τ Γ)
     → ⟦ weaken, ι (weaken, ι (s i)) ⟧ (⟨⟩ ‚ succ ⟦ n ⟧₀ ‚ ⟦ n ⟧₀)
     ≡ ⟦ s i ⟧₀
  e0 {τ} i =
   ⟦ weaken, ι (weaken, ι (s i)) ⟧ (⟨⟩ ‚ succ ⟦ n ⟧₀ ‚ ⟦ n ⟧₀)
    ≡＝⟨ ⟦weaken,-weaken,⟧ ⟨⟩ (succ ⟦ n ⟧₀) ⟦ n ⟧₀ (s i) refl (λ ()) ⟩
   ⟦ s i ⟧₀
    ∎

  e4 : {τ : type} (i : ∈Cxt τ Γ)
     → ⟦ weaken, ι (s i) ⟧ (⟨⟩ ‚ succ ⟦ n ⟧₀)
     ≡ ⟦ s i ⟧₀
  e4 {τ} i = ⟦weaken,⟧ (s i) ι _ _ (λ ())

  e1 : ⟦ close (weaken, ι (weaken, ι a)) (Subƛ (Subƛ s)) ⟧ (⟨⟩ ‚ succ ⟦ n ⟧₀ ‚ ⟦ n ⟧₀)
     ≡ ⟦ close a s ⟧₀
  e1 =
   ⟦ close (weaken, ι (weaken, ι a)) (Subƛ (Subƛ s)) ⟧ (⟨⟩ ‚ succ ⟦ n ⟧₀ ‚ ⟦ n ⟧₀)
    ≡⟨ ⟦close⟧ (weaken, ι (weaken, ι a))
               (Subƛ (Subƛ s))
               _ _
               (【≡】-is-refl‚ _ _ (【≡】-is-refl‚ _ _ (λ ()) refl) refl)
               (【≡】-【Sub】-Subƛ' _ _ _ refl refl) ⟩
   ⟦ weaken, ι (weaken, ι a) ⟧ (【Sub】 (Subƛ (Subƛ s)) (⟨⟩ ‚ succ ⟦ n ⟧₀ ‚ ⟦ n ⟧₀))
    ≡⟨ ≡-refl (weaken, ι (weaken, ι a)) (【≡】-【Sub】-Subƛ2 s (succ ⟦ n ⟧₀) ⟦ n ⟧₀ refl refl) ⟩
   ⟦ weaken, ι (weaken, ι a) ⟧ (【Sub₀】 s ‚ succ ⟦ n ⟧₀ ‚ ⟦ n ⟧₀)
    ≡⟨ ⟦weaken,-weaken,⟧ (【Sub₀】 s) (succ ⟦ n ⟧₀) ⟦ n ⟧₀ a refl (【≡】-is-refl-【Sub₀】 s) ⟩
   ⟦ a ⟧ (【Sub₀】 s)
    -- ≡＝⟨ ≡-symm (⟦close⟧' a s) ⟩
    ≡＝⟨ {!!} ⟩
   ⟦ close a s ⟧₀
    ∎

  e3 : ⟦ close (weaken, ι b) (Subƛ s) ⟧ (⟨⟩ ‚ succ ⟦ n ⟧₀) ≡ ⟦ close b s ⟧₀
  e3 =
   ⟦ close (weaken, ι b) (Subƛ s) ⟧ (⟨⟩ ‚ succ ⟦ n ⟧₀)
    ≡⟨ ⟦close⟧ (weaken, ι b)
               (Subƛ s)
               _ _
               (【≡】-is-refl‚ _ _ (λ ()) refl)
               (【≡】-【Sub】-Subƛ _ _ refl) ⟩
   ⟦ weaken, ι b ⟧ (【Sub】 (Subƛ s) (⟨⟩ ‚ succ ⟦ n ⟧₀))
    ≡⟨ ⟦weaken,⟧ b ι _ _ (【≡】-is-refl-【⊆】-⊆,-【Sub】-Subƛ s _ refl) ⟩
   ⟦ b ⟧ (【⊆】 (⊆, Γ ι) (【Sub】 (Subƛ s) (⟨⟩ ‚ succ ⟦ n ⟧₀)))
    ≡⟨ ≡-refl b e4 ⟩
   ⟦ b ⟧ (【Sub₀】 s)
    ≡＝⟨ ≡-symm (⟦close⟧' b s) ⟩
   ⟦ close b s ⟧₀
    ∎

  e6 : (i : ℕ) {τ : type} (j : ∈Cxt τ Γ)
     → ⟦ weaken, ι (weaken, ι (s j)) ⟧ (⟨⟩ ‚ succ ⟦ n ⟧₀ ‚ i)
     ≡ ⟦ s j ⟧₀
  e6 i {τ} j = ≡-trans (⟦weaken,-weaken,⟧-as-⟦weaken,⟧ ⟨⟩ i (succ ⟦ n ⟧₀) i (s j) refl (λ ()))
                       (⟦weaken,⟧ (s j) ι _ _ (λ ()))

  e5 : (i : ℕ) (u v : 〖 B-type〖 σ 〗 A 〗)
     → u ≡ v
     → ⟦ close (weaken, ι (weaken, ι a)) (Subƛ (Subƛ s)) ⟧ (⟨⟩ ‚ succ ⟦ n ⟧₀ ‚ i) (η⋆ i) u
     ≡ ⟦ weaken, ι (close a s) ⟧ (⟨⟩ ‚ i) (η⋆ i) v
  e5 i u v e =
   ⟦ close (weaken, ι (weaken, ι a)) (Subƛ (Subƛ s)) ⟧ (⟨⟩ ‚ succ ⟦ n ⟧₀ ‚ i) (η⋆ i) u
    --≡⟨ ⟦close⟧ (weaken, ι (weaken, ι a)) (Subƛ (Subƛ s)) (⟨⟩ ‚ succ ⟦ n ⟧₀ ‚ i)
    --    (【Sub】 (Subƛ (Subƛ s)) (⟨⟩ ‚ succ ⟦ n ⟧₀ ‚ i))
    --    (【≡】-is-refl‚ _ _ (【≡】-is-refl‚ _ _ (λ ()) refl) refl)
    --    (【≡】-【Sub】-Subƛ' _ _ _ refl refl)
    --    _ _ (λ a₁ b₁ a≡₁ a₂ b₂ a≡₂ → a≡₁ _ _ refl) _ _ e ⟩
    ≡⟨ {!!} ⟩
   ⟦ weaken, ι (weaken, ι a) ⟧ (【Sub】 (Subƛ (Subƛ s)) (⟨⟩ ‚ succ ⟦ n ⟧₀ ‚ i)) (η⋆ i) v
    --≡⟨ ≡-refl (weaken, ι (weaken, ι a))
    --          _ _
    --          (【≡】-【Sub】-Subƛ2 s (succ ⟦ n ⟧₀) i refl refl)
    --          _ _ {!η⋆≡η⋆ !} _ _ (≡ᵣ e) ⟩
    ≡⟨ {!!} ⟩
   ⟦ weaken, ι (weaken, ι a) ⟧ (【Sub₀】 s ‚ succ ⟦ n ⟧₀ ‚ i) (η⋆ i) v
    --≡⟨ ⟦weaken,-weaken,⟧ (【Sub₀】 s) (succ ⟦ n ⟧₀)
    --                     i a refl
    --                     (【≡】-is-refl-【Sub₀】 s)
    --                     _ _ {!η⋆≡η⋆ !} _ _ (≡ᵣ e) ⟩
    ≡⟨ {!!} ⟩
   ⟦ a ⟧ (【Sub₀】 s ) (η⋆ i) v
    --≡⟨ ≡-symm (⟦close⟧ a s (【⊆】 (∈CxtS ι) (⟨⟩ ‚ i))
    --                  (【Sub₀】 s) (λ ())
    --                  (【≡】-is-refl-【Sub₀】 s)
    --                  _ _ {! η⋆≡η⋆ !} _ _ (≡ᵣ e)) ⟩
    ≡⟨ {!!} ⟩
   ⟦ close a s ⟧ (【⊆】 (⊆, 〈〉 ι) (⟨⟩ ‚ i)) (η⋆ i) v
    --≡＝⟨ ≡-symm (⟦weaken,⟧ (close a s) ι _ _ (λ ()) _ _ {! η⋆≡η⋆ !} _ _ (≡ᵣ e)) ⟩
    ≡＝⟨ {!!} ⟩
   ⟦ weaken, ι (close a s) ⟧ (⟨⟩ ‚ i) (η⋆ i) v
    ∎

  e7 : (i j : ℕ) → i ＝ j → (u v : 〖 B-type〖 σ 〗 A 〗)
     → u ≡ v
     → ⟦ close (weaken, ι (weaken, ι a)) (Subƛ (Subƛ s)) ⟧ (⟨⟩ ‚ succ ⟦ n ⟧₀ ‚ i) (η⋆ i) u
     ≡ ⟦ weaken, ι (close a s) ⟧ (⟨⟩ ‚ j) (η⋆ j) v
  e7 i .i refl u v e = e5 i u v e

  e2 : rec (λ x → ⟦ close (weaken, ι (weaken, ι a) · (⌜η⌝ · ν₀)) (Subƛ (Subƛ s)) ⟧ (⟨⟩ ‚ succ ⟦ n ⟧₀ ‚ x))
        (⟦ close (weaken, ι b) (Subƛ s) ⟧ (⟨⟩ ‚ succ ⟦ n ⟧₀))
        ⟦ n ⟧₀
     ≡ rec ⟦ ƛ (weaken, ι (close a s) · (⌜η⌝ · ν₀)) ⟧₀ ⟦ close b s ⟧₀ ⟦ n ⟧₀
  e2 = rec-respects-≡ {_}
        {λ x → ⟦ close (weaken, ι (weaken, ι a) · (⌜η⌝ · ν₀)) (Subƛ (Subƛ s)) ⟧ (⟨⟩ ‚ succ ⟦ n ⟧₀ ‚ x)}
        {⟦ ƛ (weaken, ι (close a s) · (⌜η⌝ · ν₀)) ⟧₀}
        {⟦ close (weaken, ι b) (Subƛ s) ⟧ (⟨⟩ ‚ succ ⟦ n ⟧₀)}
        {⟦ close b s ⟧₀}
        {⟦ n ⟧₀} {⟦ n ⟧₀}
        {!!} {!!} {!!} -- e7 e3 (≡-refl₀ n)

-- as opposed to compute-Rec-Succ, this one does not "reduce" as much
compute-Rec-Succ2 : {A σ : type} {Γ : Cxt}
                        (a : T Γ (B-type〖 ι ⇒ σ ⇒ σ 〗 A))
                        (b : T Γ (B-type〖 σ 〗 A))
                        (n : T₀ ι)
                        (s : Sub₀ Γ)
                      → ⟦ close (ƛ (Rec (ƛ (weaken, ι (weaken, ι a) · (⌜η⌝ · ν₀))) (weaken, ι b) ν₀)) s  · n ⟧₀
                      ≡ ⟦ Rec (ƛ (weaken, ι (close a s) · (⌜η⌝ · ν₀))) (close b s) n ⟧₀
compute-Rec-Succ2 {A} {σ} {Γ} a b n s =
 rec (λ y → ⟦ close (weaken, ι (weaken, ι a)) (Subƛ (Subƛ s)) ⟧ (⟨⟩ ‚ ⟦ n ⟧₀ ‚ y) (η⋆ y))
     (⟦ close (weaken, ι b) (Subƛ s) ⟧ (⟨⟩ ‚ ⟦ n ⟧₀))
     ⟦ n ⟧₀
  --≡＝⟨ rec-respects-≡ {_}
  --       {λ y → ⟦ close (weaken, ι (weaken, ι a)) (Subƛ (Subƛ s)) ⟧ (⟨⟩ ‚ ⟦ n ⟧₀ ‚ y) (η⋆ y)}
  --       {λ y → ⟦ weaken, ι (close a s) ⟧ (⟨⟩ ‚ y) (η⋆ y)}
  --       {⟦ close (weaken, ι b) (Subƛ s) ⟧ (⟨⟩ ‚ ⟦ n ⟧₀)} {⟦ close b s ⟧₀}
  --       {⟦ n ⟧₀} {⟦ n ⟧₀} refl ⟩
  ≡＝⟨ {!!} ⟩
 rec (λ y → ⟦ weaken, ι (close a s) ⟧ (⟨⟩ ‚ y) (η⋆ y))
     ⟦ close b s ⟧₀
     ⟦ n ⟧₀
  ∎
 where
  e4 : (i : ℕ) {τ : type} (j : ∈Cxt τ Γ)
     → ⟦ weaken, ι (weaken, ι (s j)) ⟧ (⟨⟩ ‚ ⟦ n ⟧₀ ‚ i)
     ≡ ⟦ s j ⟧₀
  e4 i {τ} j = ⟦weaken,-weaken,⟧ ⟨⟩ ⟦ n ⟧₀ i (s j) refl (λ ())

  e3 : (i : ℕ) (u v : 〖 B-type〖 σ 〗 A 〗)
     → u ≡ v
     → ⟦ close (weaken, ι (weaken, ι a)) (Subƛ (Subƛ s)) ⟧ (⟨⟩ ‚ ⟦ n ⟧₀ ‚ i) (η⋆ i) u
     ≡ ⟦ weaken, ι (close a s) ⟧ (⟨⟩ ‚ i) (η⋆ i) v
  e3 i u v e =
   ⟦ close (weaken, ι (weaken, ι a)) (Subƛ (Subƛ s)) ⟧ (⟨⟩ ‚ ⟦ n ⟧₀ ‚ i) (η⋆ i) u
    --≡⟨ ⟦close⟧ (weaken, ι (weaken, ι a)) (Subƛ (Subƛ s)) (⟨⟩ ‚ ⟦ n ⟧₀ ‚ i)
    --    (【Sub】 (Subƛ (Subƛ s)) (⟨⟩ ‚ ⟦ n ⟧₀ ‚ i))
    --    (【≡】-is-refl‚ _ _ (【≡】-is-refl‚ _ _ (λ ()) refl) refl)
    --    (【≡】-【Sub】-Subƛ' _ _ _ refl refl)
    --    _ _ {! η⋆≡η⋆ !} _ _ e ⟩
    ≡⟨ {!!} ⟩
   ⟦ weaken, ι (weaken, ι a) ⟧ (【Sub】 (Subƛ (Subƛ s)) (⟨⟩ ‚ ⟦ n ⟧₀ ‚ i)) (η⋆ i) v
    --≡⟨ ≡-refl (weaken, ι (weaken, ι a))
    --          _ _ (【≡】-【Sub】-Subƛ2 s (⟦ n ⟧₀) i refl refl)
    --          _ _ {! η⋆ι≡ i!} _ _ (≡ᵣ e) ⟩
    ≡⟨ {!!} ⟩
   ⟦ weaken, ι (weaken, ι a) ⟧ (【Sub₀】 s ‚ ⟦ n ⟧₀ ‚ i) (η⋆ i) v
    --≡⟨ ⟦weaken,-weaken,⟧ (【Sub₀】 s) (⟦ n ⟧₀)
    --                     i a refl
    --                     (【≡】-is-refl-【Sub₀】 s)
    --                     _ _ {!η⋆ι≡ i!} _ _ (≡ᵣ e) ⟩
    ≡⟨ {!!} ⟩
   ⟦ a ⟧ (【Sub₀】 s ) (η⋆ i) v
    --≡⟨ ≡-symm (⟦close⟧ a s (【⊆】 (∈CxtS ι) (⟨⟩ ‚ i))
    --                  (【Sub₀】 s) (λ ())
    --                  (【≡】-is-refl-【Sub₀】 s)
    --                  _ _ {!η⋆ι≡ i!} _ _ (≡ᵣ e)) ⟩
    ≡⟨ {!!} ⟩
   ⟦ close a s ⟧ (【⊆】 (⊆, 〈〉 ι) (⟨⟩ ‚ i)) (η⋆ i) v
    -- ≡＝⟨ ≡-symm (⟦weaken,⟧ (close a s) ι _ _ (λ ()) _ _ {!(η⋆ι≡ i)!} _ _ (≡ᵣ e)) ⟩
    ≡＝⟨ {!!} ⟩
   ⟦ weaken, ι (close a s) ⟧ (⟨⟩ ‚ i) (η⋆ i) v
    ∎

  e5 : (i j : ℕ) → i ＝ j → (u v : 〖 B-type〖 σ 〗 A 〗)
     → u ≡ v
     → ⟦ close (weaken, ι (weaken, ι a)) (Subƛ (Subƛ s)) ⟧ (⟨⟩ ‚ ⟦ n ⟧₀ ‚ i) (η⋆ i) u
     ≡ ⟦ weaken, ι (close a s) ⟧ (⟨⟩ ‚ j) (η⋆ j) v
  e5 i .i refl u v e = e3 i u v e

  e2 : {τ : type} (i : ∈Cxt τ Γ)
     → ⟦ weaken, ι (s i) ⟧ (⟨⟩ ‚ ⟦ n ⟧₀)
     ≡ ⟦ s i ⟧₀
  e2 {τ} i = ⟦weaken,⟧ (s i) ι _ _ (λ ())

  e1 : ⟦ close (weaken, ι b) (Subƛ s) ⟧ (⟨⟩ ‚ ⟦ n ⟧₀) ≡ ⟦ close b s ⟧₀
  e1 =
   ⟦ close (weaken, ι b) (Subƛ s) ⟧ (⟨⟩ ‚ ⟦ n ⟧₀)
    ≡⟨ ⟦close⟧ (weaken, ι b) (Subƛ s)
               _ _ (【≡】-is-refl‚ _ _ (λ ()) refl)
               (【≡】-【Sub】-Subƛ _ _ refl) ⟩
   ⟦ weaken, ι b ⟧ (【Sub】 (Subƛ s) (⟨⟩ ‚ ⟦ n ⟧₀))
    ≡⟨ ⟦weaken,⟧ b ι _ _ (【≡】-is-refl-【⊆】-⊆,-【Sub】-Subƛ s _ refl) ⟩
   ⟦ b ⟧ (【⊆】 (⊆, Γ ι) (【Sub】 (Subƛ s) (⟨⟩ ‚ ⟦ n ⟧₀)))
    ≡⟨ ≡-refl b e2 ⟩
   ⟦ b ⟧ (【Sub₀】 s)
    ≡＝⟨ ≡-symm (⟦close⟧' b s) ⟩
   ⟦ close b s ⟧₀
    ∎

⟦⌜Rec⌝⟧-aux : {A : type} {σ : type} {Γ : Cxt}
              (s : 【 B-context【 Γ 】 A 】)
              (a : T Γ (ι ⇒ σ ⇒ σ))
              (b : T Γ σ)
              (a₁ b₁ : ℕ)
            → a₁ ＝ b₁
            → 【≡】-is-refl s
            → rec (λ y → ⟦ ⌜ a ⌝ ⟧ s (η⋆ y)) (⟦ ⌜ b ⌝ ⟧ s) a₁
            ≡ rec (λ y → ⟦ weaken, ι (weaken, ι ⌜ a ⌝) ⟧ (s ‚ b₁ ‚ y) (η⋆ y))
                  (⟦ weaken, ι ⌜ b ⌝ ⟧ (s ‚ b₁))
                  b₁
⟦⌜Rec⌝⟧-aux {A} {σ} {Γ} s a b a₁ b₁ a≡₁ r =
 rec-respects-≡ c (≡-symm (⟦weaken,⟧ ⌜ b ⌝ ι (s ‚ b₁) s r)) a≡₁
 where
  c : {a₂ b₂ : ℕ}
    → a₂ ＝ b₂
    → {a₃ b₃ : 〖 B-type〖 σ 〗 A 〗}
    → a₃ ≡ b₃
    → ⟦ ⌜ a ⌝ ⟧ s (η⋆ a₂) a₃
    ≡ ⟦ weaken, ι (weaken, ι ⌜ a ⌝) ⟧ (s ‚ b₁ ‚ b₂) (η⋆ b₂) b₃
  c a≡₂ a≡₃ =
   ≡-symm (⟦weaken,-weaken,⟧ s _ _ ⌜ a ⌝ refl r (η⋆≡η⋆ (≡-symm a≡₂)) (≡-symm a≡₃))

⟦⌜Rec⌝⟧ : {A : type} {σ : type} {Γ : Cxt}
          (s : 【 B-context【 Γ 】 A 】)
          (a : T Γ (ι ⇒ σ ⇒ σ))
          (b : T Γ σ)
          (c : T Γ ι)
        → 【≡】-is-refl s
        → ⟦ ⌜_⌝  {Γ} {σ} {A} (Rec a b c) ⟧ s
        ≡ ⟦ ⌜Kleisli-extension⌝ {ι} {A} {σ}
            · (ƛ (Rec (ƛ (weaken, ι (weaken, ι ⌜ a ⌝) · (⌜η⌝ · ν₀))) (weaken, ι ⌜ b ⌝) ν₀))
            · ⌜ c ⌝ ⟧ s
⟦⌜Rec⌝⟧ {A} {σ} {Γ} s a b c r =
 ⟦ ⌜_⌝  {Γ} {σ} {A} (Rec a b c) ⟧ s
  ＝≡⟨ refl ⟩
 ⟦ ⌜Kleisli-extension⌝ {ι} {A} {σ} ⟧ (s ‚ ⟦ ⌜ a ⌝ ⟧ s ‚ ⟦ ⌜ b ⌝ ⟧ s)
  (λ x → rec (λ y → ⟦ ⌜ a ⌝ ⟧ s (η⋆ y)) (⟦ ⌜ b ⌝ ⟧ s) x)
  (⟦ ⌜ c ⌝ ⟧ s)
  --≡＝⟨ ⟦⌜Kleisli-extension⌝⟧ (s ‚ ⟦ ⌜ a ⌝ ⟧ s ‚ ⟦ ⌜ b ⌝ ⟧ s) s
  --     (λ x → rec (λ y → ⟦ ⌜ a ⌝ ⟧ s (η⋆ y)) (⟦ ⌜ b ⌝ ⟧ s) x)
  --     (λ x → rec (λ y → ⟦ weaken, ι (weaken, ι ⌜ a ⌝) ⟧ (s ‚ x ‚ y) (η⋆ y)) (⟦ weaken, ι ⌜ b ⌝ ⟧ (s ‚ x)) x)
  --     (λ a₁ b₁ a≡ → ⟦⌜Rec⌝⟧-aux s a b a₁ b₁ a≡ r)
  --     (⟦ ⌜ c ⌝ ⟧ s) (⟦ ⌜ c ⌝ ⟧ s) (≡-refl ⌜ c ⌝ s s r) ⟩
  ≡＝⟨ {!!} ⟩
 ⟦ ⌜Kleisli-extension⌝ {ι} {A} {σ}
   · (ƛ (Rec (ƛ (weaken, ι (weaken, ι ⌜ a ⌝) · (⌜η⌝ · ν₀))) (weaken, ι ⌜ b ⌝) ν₀))
   · ⌜ c ⌝ ⟧ s
  ∎

⟦close-⌜Rec⌝⟧ : {A : type} {σ : type} {Γ : Cxt}
                (s : IB【 Γ 】 A)
                (a : T Γ (ι ⇒ σ ⇒ σ))
                (b : T Γ σ)
                (c : T Γ ι)
              → ⟦ close (⌜_⌝  {Γ} {σ} {A} (Rec a b c)) s ⟧₀
              ≡ ⟦ ⌜Kleisli-extension⌝ {ι} {A} {σ}
                   · close (ƛ (Rec (ƛ (weaken, ι (weaken, ι ⌜ a ⌝) · (⌜η⌝ · ν₀))) (weaken, ι ⌜ b ⌝) ν₀)) s
                   · close ⌜ c ⌝ s ⟧₀
⟦close-⌜Rec⌝⟧ {A} {σ} {Γ} s a b c =
 ⟦ close (⌜_⌝  {Γ} {σ} {A} (Rec a b c)) s ⟧₀
  ≡⟨ ⟦close⟧' ⌜ Rec a b c ⌝ s ⟩
 ⟦ ⌜_⌝  {Γ} {σ} {A} (Rec a b c) ⟧ (【Sub₀】 s)
  ≡⟨ ⟦⌜Rec⌝⟧ (【Sub₀】 s) a b c (【≡】-is-refl-【Sub₀】 s) ⟩
 ⟦ ⌜Kleisli-extension⌝ {ι} {A} {σ}
   · (ƛ (Rec (ƛ (weaken, ι (weaken, ι ⌜ a ⌝) · (⌜η⌝ · ν₀))) (weaken, ι ⌜ b ⌝) ν₀))
   · ⌜ c ⌝ ⟧ (【Sub₀】 s)
  ≡＝⟨ ≡-symm (⟦close⟧' (⌜Kleisli-extension⌝ {ι} {A} {σ}
                        · (ƛ (Rec (ƛ (weaken, ι (weaken, ι ⌜ a ⌝) · (⌜η⌝ · ν₀))) (weaken, ι ⌜ b ⌝) ν₀))
                        · ⌜ c ⌝) s) ⟩
 ⟦ close ⌜Kleisli-extension⌝ s
   · close (ƛ (Rec (ƛ (weaken, ι (weaken, ι ⌜ a ⌝) · (⌜η⌝ · ν₀))) (weaken, ι ⌜ b ⌝) ν₀)) s
   · close ⌜ c ⌝ s ⟧₀
  ＝⟨ ap (λ k → ⟦ k · close (ƛ (Rec (ƛ (weaken, ι (weaken, ι ⌜ a ⌝) · (⌜η⌝ · ν₀))) (weaken, ι ⌜ b ⌝) ν₀)) s
                    · close ⌜ c ⌝ s ⟧₀)
         ((close-⌜Kleisli-extension⌝ s) ⁻¹) ⟩
 ⟦ ⌜Kleisli-extension⌝ {ι} {A} {σ}
   · close (ƛ (Rec (ƛ (weaken, ι (weaken, ι ⌜ a ⌝) · (⌜η⌝ · ν₀))) (weaken, ι ⌜ b ⌝) ν₀)) s
   · close ⌜ c ⌝ s ⟧₀
  ∎

-- TODO maybe move this too
Rnorm-Zero : Rnorm zero' ⌜zero⌝
Rnorm-Zero {A} η₁≡η₂ β₁≡β₂ = η₁≡η₂ refl

-- TODO move the following functions probably
succ≡succ : succ ≡ succ
succ≡succ = {!!}

B⋆-functor≡B⋆-functor : {A : type}
                      → B⋆-functor ≡[ (ι ⇒ ι) ⇒ ⌜B⌝ ι A ⇒ ⌜B⌝ ι A ] B⋆-functor
B⋆-functor≡B⋆-functor f₁≡f₂ η₁≡η₂ β₁≡β₂ = η₁≡η₂ (λ n₁≡n₂ → β₁≡β₂ (f₁≡f₂ n₁≡n₂))

Rnorm-lemma : {Γ : Cxt} {σ : type}
              (xs : B【 Γ 】) (ys : {A : type} → IB【 Γ 】 A)
              (t : T Γ σ)
            → Rnorms xs ys
            → Rnorm (B⟦ t ⟧ xs) (close ⌜ t ⌝ ys)

Rnorm-lemma xs ys Zero Rnorm-xs = Rnorm-Zero

Rnorm-lemma xs ys (Succ t) Rnorm-xs =
 B⋆-functor succ ⟦ close ⌜ t ⌝ ys ⟧₀         ≡⟨ I ⟩
 B⋆-functor succ (church-encode (B⟦ t ⟧ xs)) ≡＝⟨ II ⟩
 church-encode (B-functor succ (B⟦ t ⟧ xs))  ∎
 where
  I : B⋆-functor succ ⟦ close ⌜ t ⌝ ys ⟧₀
       ≡ B⋆-functor succ (church-encode (B⟦ t ⟧ xs))
  I = B⋆-functor≡B⋆-functor succ≡succ (Rnorm-lemma xs ys t Rnorm-xs)

  II : B⋆-functor succ (church-encode (B⟦ t ⟧ xs))
        ≡ church-encode (B-functor succ (B⟦ t ⟧ xs))
  II = church-encode-is-natural (B⟦ t ⟧ xs) succ≡succ

Rnorm-lemma {Γ} {σ} γ₁ γ₂ (Rec t u v) Rnorm-γs = ?
-- Rnorm-respects-≡
--   (rec' (B⟦ t ⟧ γ₁) (B⟦ u ⟧ γ₁) (B⟦ v ⟧ γ₁))
--   (⌜Kleisli-extension⌝
--    · close (ƛ (Rec (ƛ (weaken, ι (weaken, ι ⌜ t ⌝) · (⌜η⌝ · ν₀))) (weaken, ι ⌜ u ⌝) ν₀)) γ₂
--    · close ⌜ v ⌝ γ₂)
--   (close ⌜ Rec t u v ⌝ γ₂)
--   (λ A → ≡-symm (⟦close-⌜Rec⌝⟧ {A} γ₂ t u v))
--   c1
-- where
--  rt : (x  : B〖 ι 〗) (x' : {A : type} → T₀ (B-type〖 ι 〗 A)) (rx : Rnorm {ι} x x')
--       (y  : B〖 σ 〗) (y' : {A : type} → T₀ (B-type〖 σ 〗 A)) (ry : Rnorm {σ} y y')
--     → Rnorm (B⟦ t ⟧ γ₁ x y) (close ⌜ t ⌝ γ₂ · x' · y')
--  rt = Rnorm-lemma γ₁ γ₂ t Rnorm-γs
--
--  rn : ℕ → B〖 σ 〗
--  rn n = rec (B⟦ t ⟧ γ₁ ∘ η) (B⟦ u ⟧ γ₁) n
--
--  rn' : {A : type} → T₀ (ι ⇒ B-type〖 σ 〗 A)
--  rn' = close (ƛ (Rec (ƛ (weaken, ι (weaken, ι ⌜ t ⌝) · (⌜η⌝ · ν₀))) (weaken, ι ⌜ u ⌝) ν₀)) γ₂
--
--  rnn' : (n : ℕ) → Rnorm (rn n) (rn' · numeral n)
--  rnn' zero = r
--   where
--    r : Rnorm (B⟦ u ⟧ γ₁) (rn' · Zero)
--    r = Rnorm-respects-≡
--         (B⟦ u ⟧ γ₁) (close ⌜ u ⌝ γ₂) (rn' · Zero)
--         (λ A → ≡-symm (compute-Rec-Zero {A} (ƛ (weaken, ι (weaken, ι ⌜ t ⌝) · (⌜η⌝ · ν₀))) ⌜ u ⌝ γ₂))
--         (Rnorm-lemma γ₁ γ₂ u Rnorm-γs)
--  rnn' (succ n) = r
--   where
--    r : Rnorm (B⟦ t ⟧ γ₁ (η n) (rn n)) (rn' · Succ (numeral n))
--    r = Rnorm-respects-≡
--         (B⟦ t ⟧ γ₁ (η n) (rn n))
--         (close ⌜ t ⌝ γ₂
--          · (⌜η⌝ · numeral n)
--          · Rec (ƛ (weaken, ι (close ⌜ t ⌝ γ₂) · (⌜η⌝ · ν₀))) (close ⌜ u ⌝ γ₂) (numeral n))
--         (rn' · Succ (numeral n))
--         (λ A → ≡-symm (compute-Rec-Succ {A} ⌜ t ⌝ ⌜ u ⌝ (numeral n) γ₂))
--         (rt (η n) (⌜η⌝ · numeral n) (Rnorm-ηnumeral n)
--             (rn n) (Rec (ƛ (weaken, ι (close ⌜ t ⌝ γ₂) · (⌜η⌝ · ν₀))) (close ⌜ u ⌝ γ₂) (numeral n))
--             (Rnorm-respects-≡
--               (rn n)
--               (close (ƛ (Rec (ƛ (weaken, ι (weaken, ι ⌜ t ⌝) · (⌜η⌝ · ν₀))) (weaken, ι ⌜ u ⌝) ν₀)) γ₂
--                · numeral n)
--               (Rec (ƛ (weaken, ι (close ⌜ t ⌝ γ₂) · (⌜η⌝ · ν₀))) (close ⌜ u ⌝ γ₂) (numeral n))
--               (λ A → compute-Rec-Succ2 {A} ⌜ t ⌝ ⌜ u ⌝ (numeral n) γ₂)
--               (rnn' n)))
--
--  rnn'' : (n : ℕ) (n' : T₀ ι) → Rnorm (η n) (⌜η⌝ · n') → Rnorm (rn n) (rn' · n')
--  rnn'' n n' r =
--   Rnorm-respects-≡
--    (rn n) (rn' · numeral n) (rn' · n')
--    (λ A → ≡-symm (≡-refl₀ rn' _ _ (Rnormη⌜η⌝ n n' r)))
--    (rnn' n)
--
--  c1 : Rnorm (Kleisli-extension rn (B⟦ v ⟧ γ₁))
--             (⌜Kleisli-extension⌝ · rn' · close ⌜ v ⌝ γ₂)
--  c1 = Rnorm-kleisli-lemma rn rn' rnn' (B⟦ v ⟧ γ₁) (close ⌜ v ⌝ γ₂) (Rnorm-lemma γ₁ γ₂ v Rnorm-γs)
--
Rnorm-lemma xs ys (ν i) Rnorm-γs = Rnorm-γs i

Rnorm-lemma γ₁ γ₂ (ƛ t) Rnorm-γs u₁ u₂ Rnorm-us = Rnorm-respects-≡ I IH
 where
  -- Using the semantics, we reduce application of a lambda to the appropriate
  -- substitution, at which point we can use the inductive hypothesis.
  I : {A : type} → ⟦ close ⌜ t ⌝ (Sub,, γ₂ u₂) ⟧₀ ≡[ B-type〖 _ 〗 A ] ⟦ ƛ (close ⌜ t ⌝ (Subƛ γ₂)) · u₂ ⟧₀
  I {A} = ⟦ close ⌜ t ⌝ (Sub,, γ₂ u₂) ⟧₀             ≡⟨ ⟦close⟧' ⌜ t ⌝ (Sub,, γ₂ u₂) ⟩
          ⟦ ⌜ t ⌝ ⟧ (【Sub₀】 (Sub,, γ₂ u₂))           ≡⟨ ≡-refl ⌜ t ⌝ (【≡】-【Sub】-Sub,, γ₂ u₂) ⟩
          ⟦ ⌜ t ⌝ ⟧ (【Sub】 (Subƛ γ₂) (⟨⟩ ‚ ⟦ u₂ ⟧₀)) ≡＝⟨ ≡-symm (⟦close⟧ ⌜ t ⌝ (Subƛ γ₂) _ _ (【≡】-is-refl‚ _ _ (λ ()) (≡-refl₀ u₂)) (【≡】-【Sub】-Subƛ γ₂ _ (≡-refl₀ u₂))) ⟩
          ⟦ ƛ (close ⌜ t ⌝ (Subƛ γ₂)) · u₂ ⟧₀        ∎

  Rnorm-γ,,us : Rnorms (γ₁ ‚‚ u₁) (Sub,, γ₂ u₂)
  Rnorm-γ,,us (∈Cxt0 _)   = Rnorm-us
  Rnorm-γ,,us (∈CxtS _ i) = Rnorm-γs i

  IH : Rnorm (B⟦ t ⟧ (γ₁ ‚‚ u₁)) (close ⌜ t ⌝ (Sub,, γ₂ u₂))
  IH = Rnorm-lemma (γ₁ ‚‚ u₁) (Sub,, γ₂ u₂) t Rnorm-γ,,us

Rnorm-lemma γ₁ γ₂ (t · u) Rnorm-γs = IH₁ (B⟦ u ⟧ γ₁) (close ⌜ u ⌝ γ₂) IH₂
 where
  IH₁ : Rnorm (B⟦ t ⟧ γ₁) (close ⌜ t ⌝ γ₂)
  IH₁ = Rnorm-lemma γ₁ γ₂ t Rnorm-γs

  IH₂ : Rnorm (B⟦ u ⟧ γ₁) (close ⌜ u ⌝ γ₂)
  IH₂ = Rnorm-lemma γ₁ γ₂ u Rnorm-γs

---- a consequence of Rnorm-lemma for terms of type ι
--Rnorm-lemmaι : (t : T₀ ι) (α : Baire)
--             → dialogue⋆ ⟦ ⌜ t ⌝ ⟧₀ ≡ dialogue⋆ (church-encode B⟦ t ⟧₀)
--Rnorm-lemmaι t α =
-- dialogue⋆ ⟦ ⌜ t ⌝ ⟧₀
--  ≡⟨ ≡-symm (⟦closeν⟧ ⌜ t ⌝ _ (λ ()) _ _ η≡ _ _ β≡) ⟩
-- dialogue⋆ ⟦ close ⌜ t ⌝ ν ⟧₀
--  ≡＝⟨ Rnorm-lemma ⟪⟫ ν t (λ ()) ((ι ⇒ ι) ⇒ ι) η' β' eη eβ ⟩
-- dialogue⋆ (church-encode B⟦ t ⟧₀)
--  ∎
-- where
--  η' : ℕ → Baire → ℕ
--  η' = λ z α → z
--
--  β' : (ℕ → Baire → ℕ) → ℕ → Baire → ℕ
--  β' = λ φ x α → φ (α x) α
--
--  η≡ : η' ≡ η'
--  η≡ a b a≡ a₁ b₁ a≡₁ = a≡
--
--  β≡ : β' ≡ β'
--  β≡ a b a≡ a₁ b₁ a≡₁ a₂ b₂ a≡₂ = a≡ _ _ (a≡₂ _ _ a≡₁) _ _ a≡₂
--
--  eη : extη η'
--  eη x a b a≡ = refl
--
--  eβ : extβ β'
--  eβ a b x .x refl a≡ a₁ b₁ a≡₁ =
--   a≡ _ _ _ a≡₁ ∙ a≡b _ _ (a≡₁ _ _ refl ⁻¹) ⁻¹ ∙ a≡ _ _ _ a≡₁
--   where
--    a≡b : (n m : ℕ) → n ＝ m → a n a₁ ＝ b m b₁
--    a≡b n .n refl = a≡ _ _ _ a≡₁
--
--Rnorm-lemma₀ : {σ : type} (t : T₀ σ) → Rnorm B⟦ t ⟧₀ ⌜ t ⌝
--Rnorm-lemma₀ {σ} t =
-- Rnorm-respects-≡
--  B⟦ t ⟧₀ (close ⌜ t ⌝ ν) ⌜ t ⌝
--  (λ A → ⟦closeν⟧ ⌜ t ⌝ _ (λ ()))
--  (Rnorm-lemma ⟪⟫ ν t (λ ()))
--
--Rnorm-generic : (u : B ℕ) (u' : {A : type} → T₀ (⌜B⌝ ι A))
--              → is-dialogue-for u u'
--              → is-dialogue-for (generic u) (⌜generic⌝ · u')
--Rnorm-generic u u' ru =
-- Rnorm-kleisli-lemma (β η) (⌜β⌝ · ⌜η⌝) c u u' ru
-- where
--  c : (x : ℕ)
--    → β⋆ η⋆ ⟦ numeral x ⟧₀ ≣⋆ β⋆ η⋆ x
--  c x A η' β' eη eβ = eβ _ _ _ _ (⟦numeral⟧ x) eη
--
--⌜dialogue-tree⌝-correct : (t : T₀ ((ι ⇒ ι) ⇒ ι))
--                          (α : Baire)
--                        → ⟦ t ⟧₀ α ＝ dialogue⋆ ⟦ ⌜dialogue-tree⌝ t ⟧₀ α
--⌜dialogue-tree⌝-correct t α =
-- dialogue-tree-correct t α
-- ∙ dialogues-agreement (dialogue-tree t) α
-- ∙ e ⁻¹
-- where
--  η' : ℕ → Baire → ℕ
--  η' = λ z i → z
--
--  β' : (ℕ → Baire → ℕ) → ℕ → Baire → ℕ
--  β' = λ φ x α → φ (α x) α
--
--  rt : Rnorm B⟦ t ⟧₀ ⌜ t ⌝
--  rt = Rnorm-lemma₀ {(ι ⇒ ι) ⇒ ι} t
--
--  eη : extη η'
--  eη x a b a≡ = refl
--
--  eβ : extβ β'
--  eβ f g x .x refl f≡ a b a≡ =
--   f≡ _ _ _ a≡ ∙ a≡b _ _ (a≡ _ _ refl ⁻¹) ⁻¹ ∙ f≡ _ _ _ a≡
--   where
--    a≡b : (n m : ℕ) → n ＝ m → f n a ＝ g m b
--    a≡b n .n refl = f≡ _ _ _ a≡
--
--  eα : (a b : ℕ) → a ＝ b → α a ＝ α b
--  eα a .a refl = refl
--
--  e : ⟦ ⌜ t ⌝ · ⌜generic⌝ ⟧₀ η' β' α ≡ church-encode (B⟦ t ⟧₀ generic) η' β' α
--  e = rt generic ⌜generic⌝ Rnorm-generic ((ι ⇒ ι) ⇒ ι) η' β' eη eβ _ _ eα
--
--⌜dialogue⌝ : {Γ : Cxt}
--           → T (B-context【 Γ 】 ((ι ⇒ ι) ⇒ ι)) (⌜B⌝ ι ((ι ⇒ ι) ⇒ ι))
--           → T (B-context【 Γ 】 ((ι ⇒ ι) ⇒ ι)) ((ι ⇒ ι) ⇒ ι)
--⌜dialogue⌝ {Γ} t = t · ƛ (ƛ ν₁) · ƛ (ƛ (ƛ (ν₂ · (ν₀ · ν₁) · ν₀)))
--
---- Same as ⌜dialogue-tree⌝-correct but using an internal dialogue function
--⌜dialogue-tree⌝-correct' : (t : T₀ ((ι ⇒ ι) ⇒ ι))
--                           (α : Baire)
--                         → ⟦ t ⟧₀ α ＝ ⟦ ⌜dialogue⌝ (⌜dialogue-tree⌝ t) ⟧₀ α
--⌜dialogue-tree⌝-correct' t α = ⌜dialogue-tree⌝-correct t α

\end{code}
